WIP update grammar

compiler.v
@@ -1,32 +1,83 @@
-(** * Transform Language *)
+
+(** * Compiler Logic *)
 Set Warnings "-notation-overridden,-parsing".
 From LF Require Import imports.
 From LF Require Import transforms.
 From LF Require Import python.
 
-Fixpoint numExprCompile (ae : AbNumExpr) : PyNumExpr :=
+Fixpoint numCompile (ae : AbNum) : PyNum :=
   match ae with
     | AbLit l => PyLit l
     | AbId n => PyId n
   end.
 
-Fixpoint compile (ac : AbCommand) : PyCommand :=
-  match ac with
-    | AbSkip => PyNewLine
-    | AbAssign x a => PyAssign x (numExprCompile a)
-    | AbSeq c1 c2 => PySeq (compile c1) (compile c2)
-    | AbEnclosed c1 => compile c1
+Fixpoint numExprCompile (ae : AbNumExpr) : PyNumExpr :=
+  match ae with
+    | AbNum2 n => PyNum2 (numCompile n)
+    | AbAdd a1 a2 => PyAdd (numExprCompile a1) (numExprCompile a2)
+    | AbSub a1 a2 => PySub (numExprCompile a1) (numExprCompile a2)
+    | AbMulti a1 a2 => PyMulti (numExprCompile a1) (numExprCompile a2)
   end.
 
-Compute compile (AbAssign "x" (AbLit 3)).
+Fixpoint exprCompile (e : AbExpr) : PyExpr :=
+  match e with
+    | Ab_Num_Expr n => Py_Num_Expr (numExprCompile n)
+  end.
+
+Fixpoint compile (ac : AbCommand) : PyCommand :=
+  match ac with
+  | AbTransform x a => PyAssign x (exprCompile a)
+  | AbSeq c1 c2 => PySeq (compile c1) (compile c2)
+  end.
+
+Compute compile (AbTransform "x" (Ab_Num_Expr (AbNum2 (AbLit 3)))).
+
+Theorem numEquiv : forall ab st,
+    AbEvalNumVal st ab = PyEvalNumVal st (numCompile ab).
+Proof.
+  intros; induction ab; reflexivity.
+Qed.
+
+Theorem numExprEquiv : forall ab st,
+    AbEvalNum st ab = PyEvalNum st (numExprCompile ab).
+Proof.
+  intros.
+  induction ab;
+    (* Handles cases for AbAdd, AbSub, AbMulti *)
+    try ( induction ab1; induction ab2; simpl in *; rewrite IHab1; rewrite IHab2; reflexivity ).
+  - (* AbNum2 -> PyNum2 *)
+    induction n; reflexivity.
+Qed.
+
+Theorem exprEquiv : forall ab st,
+    AbEval st ab = PyEval st (exprCompile ab).
+Proof.
+  intros. induction ab. apply numExprEquiv.
+Qed.
 
 Theorem compiler_correctness : forall a st st1 st2,
-    (AbExec a st st1) ->
-    (PyExec (compile a) st st2) ->
+    (AbInitioProgram a st st1) ->
+    (PythonProgram (compile a) st st2) ->
     st1 = st2.
 Proof.
   intros.
-  induction a; simpl in *; inversion H; inversion H0; subst.
+
+
+
+
+
+  
+  induction a.
+  - (* AbTransform -> PyAssign *)
+    induction a.
+    * (* AbNum2 -> PyNum2 *)
+      simpl in *.
+      
+      inversion H; inversion H0; subst. reflexivity.
+    * (* AbAdd -> PyAdd *)
+      inversion H. inversion H0. subst. .
+      apply IHa1.
+      + apply H.
   - (* AbSkip -> PyNewLine*) reflexivity.
   - (* AbAssign -> PyAssign *) induction a; simpl; reflexivity.
   - (* AbSeq -> PySeq *) apply IHa1.
