transforms.v
@@ -3,12 +3,12 @@
 Set Warnings "-notation-overridden,-parsing".
 From LF Require Import imports.
 
-(* Expressions that result in a nat *)
+(* Values that result in a nat *)
 Inductive AbNum : Type :=
   | AbLit (n : nat)
   | AbId (s : string).
 
-(* Expressions that result in a bool *)
+(* Values that result in a bool *)
 Inductive AbBinExpr : Type :=
   | BinTrue
   | BinFalse.
@@ -20,16 +20,17 @@ Inductive AbNumExpr : Type :=
   | AbSub (a1 : AbNumExpr) (a2 : AbNumExpr)
   | AbMulti (a1 : AbNumExpr) (a2 : AbNumExpr).
 
+(* Expressions from the transform language *)
+Inductive AbExpr : Type :=
+  | Ab_Num_Expr (a : AbNumExpr).
+
 (* Commands from the transform language *)
 Inductive AbCommand : Type :=
-  | AbSkip
-  | AbAssign (x : string) (a : AbNumExpr)
-  | AbNumExpr2 (e : AbNumExpr)
-  | AbSeq (c1 : AbCommand) (c2 : AbCommand)
-  | AbEnclosed (c1 : AbCommand).
+  | AbTransform (x : string) (a : AbExpr)
+  | AbSeq (c1 c2 : AbCommand).
 
 (* Evaluation of numerical values *)
-Fixpoint AbEvalVal (st : state) (a : AbNum) : nat :=
+Fixpoint AbEvalNumVal (st : state) (a : AbNum) : nat :=
   match a with
   | AbLit l => l
   | AbId n => st n
@@ -38,7 +39,7 @@ Fixpoint AbEvalVal (st : state) (a : AbNum) : nat :=
 (* Evaluation of numerical expressions *)
 Fixpoint AbEvalNum (st : state) (a : AbNumExpr) : nat :=
   match a with
-  | AbNum2 n => AbEvalVal st n
+  | AbNum2 n => AbEvalNumVal st n
   | AbAdd a1 a2 => (AbEvalNum st a1) + (AbEvalNum st a2)
   | AbSub a1 a2 => (AbEvalNum st a1) - (AbEvalNum st a2)
   | AbMulti a1 a2 => (AbEvalNum st a1) * (AbEvalNum st a2)
@@ -51,21 +52,20 @@ Fixpoint AbBinEval (st : state) (b : AbBinExpr) : bool :=
   | BinFalse => false
   end.
 
+(* TODO allow bools to be returned *)
+(* Evaluation of expressions *)
+Fixpoint AbEval (st : state) (a : AbExpr) : nat :=
+  match a with
+  | Ab_Num_Expr a => AbEvalNum st a
+  end.
+
 (* Execution of commands *)
-Inductive AbExec : AbCommand -> state -> state -> Prop :=
-  | Ab_Skip : forall st,
-      AbSkip / st \\ st
-  | Ab_Assign  : forall st a1 n x,
+Inductive AbInitioProgram : AbCommand -> state -> state -> Prop :=
+  | Ab_Transform  : forall st a1 n x,
       AbEvalNum st a1 = n ->
-      (AbAssign x a1) / st \\ st & { x --> n }
-  | Ab_Add  : forall st e n,
-      AbEvalNum st e = n ->
-      (AbNumExpr2 e) / st \\ st
+      (AbTransform x (Ab_Num_Expr (AbNum2 (AbLit n)))) / st \\ st & { x --> n }
   | Ab_Seq : forall c1 c2 st st' st'',
       c1 / st \\ st' ->
       c2 / st' \\ st'' ->
       (AbSeq c1 c2) / st \\ st''
-  | Ab_Enclosed : forall c1 st st',
-      c1 / st \\ st' ->
-      (AbEnclosed c1) / st \\ st'
-  where "c1 '/' st '\\' st'" := (AbExec c1 st st').
+  where "c1 '/' st '\\' st'" := (AbInitioProgram c1 st st').
